Clean-up

code/ecdsa/Hacl.Impl.EC.PointAdd.fst
@@ -18,8 +18,6 @@ open FStar.Tactics.Canon
 
 open FStar.Math.Lemmas
 open Hacl.Impl.EC.Masking
-open Hacl.Spec.EC.Definition
-
 
 open Hacl.Spec.MontgomeryMultiplication
 open FStar.Mul
@@ -32,13 +30,13 @@ open Hacl.Impl.P.PointAdd.Aux
 inline_for_extraction noextract
 val copy_point_conditional: #c: curve -> x3_out: felem c -> y3_out: felem c -> z3_out: felem c -> p: point c -> mask: point c ->
   Stack unit
-  (requires fun h -> 
+  (requires fun h -> point_eval c h mask /\ point_eval c h p /\
     live h x3_out /\ live h y3_out /\ live h z3_out /\ live h p /\ live h mask /\ 
     LowStar.Monotonic.Buffer.all_disjoint [loc x3_out; loc y3_out; loc z3_out; loc p; loc mask])
   (ensures fun h0 _ h1 -> modifies (loc x3_out |+| loc y3_out |+| loc z3_out) h0 h1 /\ (
     let mask = point_z_as_nat c h0 mask in 
     let x, y, z = point_x_as_nat c h0 p, point_y_as_nat c h0 p, point_z_as_nat c h0 p in
-    if mask = 0 then 
+    if mask = 0 then
       as_nat c h1 x3_out == x /\
       as_nat c h1 y3_out == y /\ 
       as_nat c h1 z3_out == z
@@ -50,7 +48,7 @@ val copy_point_conditional: #c: curve -> x3_out: felem c -> y3_out: felem c -> z
 
 let copy_point_conditional #c x3_out y3_out z3_out p maskPoint = 
   [@inline_let]
-  let len  = getCoordinateLenU64 c in 
+  let len = getCoordinateLenU64 c in 
   
   let z = sub maskPoint (size 2 *! len) len in 
   let mask = isZero_uint64_CT #c z in 
@@ -195,41 +193,6 @@ let move_from_jacobian_coordinates #c p q t12 =
   _move_from_jacobian_coordinates #c u1 u2 s1 s2 p q t4
 
 
-
-inline_for_extraction noextract 
-val _compute_common_params_point_add: #c: curve -> h: felem c -> r: felem c -> uh: felem c -> 
-  hCube: felem c -> u1: felem c -> u2: felem c -> s1: felem c -> s2: felem c -> 
-  t4: lbuffer uint64 (size 4 *! getCoordinateLenU64 c) -> 
-  Stack unit (requires fun h0 -> 
-    live h0 h /\ live h0 r /\ live h0 uh /\ live h0 hCube /\ live h0 t4 /\ 
-    live h0 u1 /\ live h0 u2 /\ live h0 s1 /\ live h0 s2 /\
-    LowStar.Monotonic.Buffer.all_disjoint [loc u1; loc u2; loc s1; loc s2; loc h; loc r; loc uh; loc hCube; loc t4] /\ 
-    felem_eval c h0 u1 /\ felem_eval c h0 u2 /\ felem_eval c h0 s1 /\ felem_eval c h0 s2)
-  (ensures fun h0 _ h1 -> 
-    modifies (loc h |+| loc r |+| loc uh |+| loc hCube |+| loc t4) h0 h1 /\
-    hInvariant #c h1 h u1 u2 /\
-    rInvariant #c h1 r s1 s2 /\
-    uhInvariant #c h1 uh h u1 /\
-    hCubeInvariant #c h1 hCube h
-  )
-
-
-let _compute_common_params_point_add #c h r uh hCube u1 u2 s1 s2 t4 =  
-  [@inline_let]
-  let len = getCoordinateLenU64 c in
-  let temp = sub t4 (size 0) len in 
-  
-  felem_sub u2 u1 h; 
-  felem_sub s2 s1 r;    
-  montgomery_square_buffer_dh h temp;
-    let h1 = ST.get() in   
-  montgomery_multiplication_buffer_dh temp u1 uh;
-  montgomery_multiplication_buffer_dh temp h hCube;
-
-  let prime = getPrime c in 
-  lemma_mod_mul_distr_l (fromDomain #c (as_nat c h1 h) * fromDomain #c (as_nat c h1 h)) (fromDomain #c (as_nat c h1 u1)) prime;
-  lemma_mod_mul_distr_l (fromDomain #c (as_nat c h1 h) * fromDomain #c (as_nat c h1 h)) (fromDomain #c (as_nat c h1 h)) prime
-
 inline_for_extraction noextract
 val compute_common_params_point_add: #c: curve 
   -> t12: lbuffer uint64 (size 12 *! getCoordinateLenU64 c) -> 
@@ -256,7 +219,7 @@ let compute_common_params_point_add #c t12 =
   let len = getCoordinateLenU64 c in
   lemma_ICuttable_common #c; 
 
-  let t4 = sub t12 (size 0) (size 4 *! len) in 
+  let temp = sub t12 (size 0) len in 
 
   let u1 = sub t12 (size 4 *! len) len in 
   let u2 = sub t12 (size 5 *! len) len in 
@@ -268,35 +231,44 @@ let compute_common_params_point_add #c t12 =
   let uh = sub t12 (size 10 *! len) len in
   let hCube = sub t12 (size 11 *! len) len in 
 
-  _compute_common_params_point_add #c h r uh hCube u1 u2 s1 s2 t4
+  felem_sub #c u2 u1 h; 
+  felem_sub #c s2 s1 r;    
+  montgomery_square_buffer_dh #c h temp;
+    let h1 = ST.get() in   
+  montgomery_multiplication_buffer_dh #c temp u1 uh;
+  montgomery_multiplication_buffer_dh #c temp h hCube;
+
+  let prime = getPrime c in 
+  lemma_mod_mul_distr_l (fromDomain #c (as_nat c h1 h) * fromDomain #c (as_nat c h1 h)) (fromDomain #c (as_nat c h1 u1)) prime;
+  lemma_mod_mul_distr_l (fromDomain #c (as_nat c h1 h) * fromDomain #c (as_nat c h1 h)) (fromDomain #c (as_nat c h1 h)) prime
 
 
 inline_for_extraction noextract
-val _computeX3_point_add: #c : curve -> x3: felem c -> hCube: felem c -> uh: felem c -> 
-  r: felem c -> t3: lbuffer uint64 (size 3 *! getCoordinateLenU64 c) ->  
+val computex3_point_add: #c : curve -> hCube: felem c -> uh: felem c -> 
+  r: felem c -> t5: lbuffer uint64 (size 5 *! getCoordinateLenU64 c) ->  
   Stack unit 
   (requires fun h0 -> 
-    live h0 x3 /\ live h0 hCube /\ live h0 uh /\ live h0 r /\ live h0 r /\ live h0 t3 /\
-    disjoint hCube t3 /\  disjoint uh t3 /\  disjoint x3 t3 /\ disjoint r t3 /\ 
-    disjoint x3 r /\ disjoint x3 hCube /\ disjoint x3 uh /\
+    live h0 hCube /\ live h0 uh /\ live h0 r /\ live h0 t5 /\
+    disjoint hCube t5 /\ disjoint uh t5 /\ disjoint r t5 /\
     felem_eval c h0 hCube /\ felem_eval c h0 uh /\ felem_eval c h0 r)
-  (ensures fun h0 _ h1 -> 
-    modifies (loc x3 |+| loc t3) h0 h1 /\ x3Invariant #c h0 h1 x3 r hCube uh)
+  (ensures fun h0 _ h1 -> modifies (loc t5) h0 h1 /\ (
+    let x3 = gsub t5 (size 0) (getCoordinateLenU64 c) in
+    x3Invariant #c h0 h1 x3 r hCube uh))
 
-
-let _computeX3_point_add #c x3 hCube uh r t3 = 
-  let h0 = ST.get() in
+let computex3_point_add #c hCube uh r t4 = 
+    let h0 = ST.get() in
   [@inline_let]
   let len = getCoordinateLenU64 c in 
   
-  let rSquare = sub t3 (size 0) len in 
-  let rH = sub t3 len len in 
-  let twoUh = sub t3 (size 2 *! len) len in 
+  let x3 = sub t4 (size 0) len in 
+  let rSquare = sub t4 len len in 
+  let rH = sub t4 (size 2 *! len) len in 
+  let twoUh = sub t4 (size 3 *! len) len in 
   
   montgomery_square_buffer_dh r rSquare; 
   felem_sub rSquare hCube rH;
   multByTwo uh twoUh;
-  felem_sub rH twoUh x3; 
+  felem_sub #c rH twoUh x3; 
 
   let prime = getPrime c in 
   let r = as_nat c h0 r in 
@@ -318,66 +290,44 @@ let _computeX3_point_add #c x3 hCube uh r t3 =
     toDomain ((fromDomain r * fromDomain r - fromDomain (as_nat h0 hCube) - 2 * fromDomain (as_nat h0 uh)) % prime);
   }
 
+
 inline_for_extraction noextract
-val computex3_point_add: #c : curve -> hCube: felem c -> uh: felem c -> 
-  r: felem c -> t5: lbuffer uint64 (size 5 *! getCoordinateLenU64 c) ->  
+val computeY3_point_add: #c: curve -> s1: felem c -> hCube: felem c -> uh: felem c -> r: felem c 
+  -> t5: lbuffer uint64 (size 5 *! getCoordinateLenU64 c) -> 
   Stack unit 
-  (requires fun h0 -> 
-    live h0 hCube /\ live h0 uh /\ live h0 r /\ live h0 t5 /\
-    disjoint hCube t5 /\ disjoint uh t5 /\ disjoint r t5 /\
-    felem_eval c h0 hCube /\ felem_eval c h0 uh /\ felem_eval c h0 r)
+  (requires fun h -> 
+    let x3_out = gsub t5 (size 0) (getCoordinateLenU64 c) in 
+    live h s1 /\ live h hCube /\ live h uh /\ live h r /\ live h t5 /\
+    disjoint uh t5 /\ disjoint r t5 /\ disjoint s1 t5 /\ disjoint hCube t5 /\ 
+    eq_or_disjoint s1 hCube /\ 
+    felem_eval c h s1 /\ felem_eval c h hCube /\ felem_eval c h uh /\ felem_eval c h x3_out /\ felem_eval c h r)
   (ensures fun h0 _ h1 -> 
-    let x3 = gsub t5 (size 0) (getCoordinateLenU64 c) in 
-    modifies (loc t5) h0 h1 /\ 
-    x3Invariant #c h0 h1 x3 r hCube uh)
+    let len = getCoordinateLenU64 c in 
+    let x3_out = gsub t5 (size 0) len in 
+    let y3_out = gsub t5 len len in 
+    modifies (loc t5) h0 h1 /\
+    as_nat c h0 x3_out == as_nat c h1 x3_out /\
+    y3Invariant #c h0 h1 y3_out s1 hCube uh x3_out r)
 
+let computeY3_point_add #c s1 hCube uh r tempBuffer5 = 
+  let x3 = sub tempBuffer5 (size 0) (getCoordinateLenU64 c) in 
+  let y3 = sub tempBuffer5 (getCoordinateLenU64 c) (getCoordinateLenU64 c) in 
 
-let computex3_point_add #c hCube uh r t4 = 
-  [@inline_let]
-  let len = getCoordinateLenU64 c in 
-  
-  let x3 = sub t4 (size 0) len in 
-  let tempBuffer3 = sub t4 len (size 3 *! len) in 
-  _computeX3_point_add x3 hCube uh r tempBuffer3
-
-
-inline_for_extraction noextract 
-val _computeY3_point_add: #c: curve -> y3: felem c -> s1: felem c -> 
-  hCube: felem c -> uh: felem c -> x3_out: felem c -> r: felem c -> 
-  t3: lbuffer uint64 (size 3 *! getCoordinateLenU64 c) -> 
-  Stack unit 
-    (requires fun h -> 
-      live h y3 /\ live h s1 /\ live h hCube /\ live h uh /\ live h uh /\ live h x3_out /\ live h r /\ live h t3 /\
-      disjoint uh t3 /\ disjoint x3_out t3 /\  disjoint y3 t3 /\
-      disjoint r t3 /\
-      disjoint s1 t3 /\
-      disjoint hCube t3 /\ 
-
-      disjoint y3 s1 /\ disjoint y3 hCube /\ disjoint y3 uh /\ disjoint y3 x3_out /\ disjoint y3 r /\
-      
-      felem_eval c h s1 /\ felem_eval c h hCube /\ felem_eval c h uh /\ felem_eval c h x3_out /\ 
-      felem_eval c h r)
-    (ensures fun h0 _ h1 ->
-      modifies (loc y3 |+| loc t3) h0 h1 /\ y3Invariant #c h0 h1 y3 s1 hCube uh x3_out r)
-      
-
-let _computeY3_point_add #c y3 s1 hCube uh x3 r t3 = 
   let h0 = ST.get() in
 
   [@inline_let]
   let len = getCoordinateLenU64 c in 
   
-  let s1hCube = sub t3 (size 0) len in 
-  let u1hx3 = sub t3 len len in 
-  let ru1hx3 = sub t3 (size 2 *! len) len in 
-
+  let s1hCube = sub tempBuffer5 (size 2 *! getCoordinateLenU64 c) len in 
+  let u1hx3 = sub tempBuffer5 (size 3 *! getCoordinateLenU64 c) len in 
+  let ru1hx3 = sub tempBuffer5 (size 4 *! getCoordinateLenU64 c) len in 
+  
   montgomery_multiplication_buffer_dh s1 hCube s1hCube;
   felem_sub uh x3 u1hx3; 
   montgomery_multiplication_buffer_dh u1hx3 r ru1hx3; 
   felem_sub #c ru1hx3 s1hCube y3;
 
   let h3 = ST.get() in 
-
 
   let prime = getPrime c in
 
@@ -400,66 +350,6 @@ let _computeY3_point_add #c y3 s1 hCube uh x3 r t3 =
     toDomain #c (((uhD - x3D) * rD - s1D * hCubeD) % getPrime c);
   }
 
-inline_for_extraction noextract
-val computeY3_point_add: #c: curve -> s1: felem c -> hCube: felem c -> uh: felem c -> r: felem c -> 
-  t5: lbuffer uint64 (size 5 *! getCoordinateLenU64 c) -> 
-  Stack unit 
-    (requires fun h -> 
-      let x3_out = gsub t5 (size 0) (getCoordinateLenU64 c) in 
-      live h s1 /\ live h hCube /\ live h uh /\ live h r /\ live h t5 /\
-      
-      disjoint uh t5 /\
-      disjoint r t5 /\
-      disjoint s1 t5 /\
-      disjoint hCube t5 /\ 
-      
-      felem_eval c h s1 /\ 
-      felem_eval c h hCube /\
-      felem_eval c h uh /\ 
-      felem_eval c h x3_out /\ 
-      felem_eval c h r)
-    (ensures fun h0 _ h1 -> 
-      let len = getCoordinateLenU64 c in 
-      let x3_out = gsub t5 (size 0) len in 
-      let y3_out = gsub t5 len len in 
-      modifies (loc t5) h0 h1 /\
-      as_nat c h0 x3_out == as_nat c h1 x3_out /\
-      y3Invariant #c h0 h1 y3_out s1 hCube uh x3_out r)
-
-
-let computeY3_point_add #c s1 hCube uh r tempBuffer5 = 
-  let x3 = sub tempBuffer5 (size 0) (getCoordinateLenU64 c) in 
-  let y3 = sub tempBuffer5 (getCoordinateLenU64 c) (getCoordinateLenU64 c) in 
-  let tempBuffer3 = sub tempBuffer5 (size 2 *! getCoordinateLenU64 c) (size 3 *! getCoordinateLenU64 c) in 
-  _computeY3_point_add #c y3 s1 hCube uh x3 r tempBuffer3
-
-
-
-inline_for_extraction noextract 
-val __computeZ3_point_add: #c: curve -> z3: felem  c ->  z1: felem c -> z2: felem c ->
-  h: felem c -> tempBuffer: felem c -> 
-  Stack unit
-  (requires fun h0 -> 
-    live h0 z3 /\ live h0 z1 /\ live h0 z2 /\ live h0 h /\  live h0 tempBuffer /\
-    disjoint z3 z1 /\ disjoint z1 tempBuffer /\ disjoint tempBuffer h /\
-    disjoint h z3 /\ disjoint z2 tempBuffer /\ disjoint z3 z2 /\
-    felem_eval c h0 z1 /\ felem_eval c h0 z2 /\ felem_eval c h0 h)
-  (ensures fun h0 _ h1 ->
-    modifies (loc z3 |+| loc tempBuffer) h0 h1 /\ 
-    z3Invariant #c h0 h1 z3 z1 z2 h)  
-
-
-let __computeZ3_point_add #c z3 z1 z2 h tempBuffer = 
-  let h0 = ST.get() in 
-  let z1z2 = sub tempBuffer (size 0) (getCoordinateLenU64 c) in
-  montgomery_multiplication_buffer_dh z1 z2 z1z2;
-  montgomery_multiplication_buffer_dh z1z2 h z3;
-
-  calc (==)
-  {
-    toDomain #c ((fromDomain #c (as_nat c h0 z1) * fromDomain #c (as_nat c h0 z2) % getPrime c) * fromDomain #c (as_nat c h0 h) % getPrime c);
-    (==) {lemma_mod_mul_distr_l (fromDomain #c (as_nat c h0 z1) * fromDomain #c (as_nat c h0 z2)) (fromDomain #c (as_nat c h0 h)) (getPrime c)}
-    toDomain #c (fromDomain #c (as_nat c h0 z1) * fromDomain #c (as_nat c h0 z2) * fromDomain #c (as_nat c h0 h) % getPrime c);}
 
 
 inline_for_extraction noextract 
@@ -468,57 +358,62 @@ val computeZ3_point_add: #c: curve -> p: point c -> q: point c ->
   Stack unit 
   (requires fun h0 -> 
     live h0 t5 /\ live h0 p /\ live h0 q /\ live h0 h /\ 
-    disjoint t5 p /\ disjoint t5 h /\ disjoint t5 q /\
+    disjoint t5 p /\ disjoint t5 h /\ disjoint t5 q /\ eq_or_disjoint p q /\
     point_eval c h0 p /\ point_eval c h0 q /\ felem_eval c h0 h)
-  (ensures fun h0 _ h1 ->     
-    modifies (loc t5) h0 h1 /\ (
+  (ensures fun h0 _ h1 -> modifies (loc t5) h0 h1 /\ (
     let len = getCoordinateLenU64 c in 
-    let z1 = getZ p in 
-    let z2 = getZ q in 
-    
+    let z1, z2 = getZ p, getZ q in 
     let x3, y3, z3 = getXYZ #c t5 in 
-    
     as_nat c h0 x3 == as_nat c h1 x3 /\
     as_nat c h0 y3 == as_nat c h1 y3 /\
     z3Invariant #c h0 h1 z3 z1 z2 h))
 
 let computeZ3_point_add #c p q h t5 = 
+    let h0 = ST.get() in 
   [@inline_let]
   let len = getCoordinateLenU64 c in 
 
   let z1 = sub p (size 2 *! len) len in 
   let z2 = sub q (size 2 *! len) len in 
   let z3 = sub t5 (size 2 *! len) len in 
-  let t1 = sub t5 (size 3 *! len) len in 
+  
+  let z1z2 = sub t5 (size 3 *! len) len in 
 
-  __computeZ3_point_add z3 z1 z2 h t1
+  montgomery_multiplication_buffer_dh #c z1 z2 z1z2;
+  montgomery_multiplication_buffer_dh #c z1z2 h z3;
+
+  calc (==)
+  {
+    toDomain #c ((fromDomain #c (as_nat c h0 z1) * fromDomain #c (as_nat c h0 z2) % getPrime c) * fromDomain #c (as_nat c h0 h) % getPrime c);
+    (==) {lemma_mod_mul_distr_l (fromDomain #c (as_nat c h0 z1) * fromDomain #c (as_nat c h0 z2)) (fromDomain #c (as_nat c h0 h)) (getPrime c)}
+    toDomain #c (fromDomain #c (as_nat c h0 z1) * fromDomain #c (as_nat c h0 z2) * fromDomain #c (as_nat c h0 h) % getPrime c);}
+
+
 
 inline_for_extraction noextract
 val copy_result_point_add: #c: curve 
   -> t5: lbuffer uint64 (size 5 *! (getCoordinateLenU64 c)) 
   -> p: point c -> q: point c -> result: point c ->
   Stack unit 
-    (requires fun h -> live h t5 /\ live h p /\ live h q /\ live h result /\
-      eq_or_disjoint p result /\
-      disjoint t5 result /\
-      LowStar.Monotonic.Buffer.all_disjoint [loc t5; loc p; loc q]
-    )
-    (ensures fun h0 _ h1 -> 
-      let x3_out, y3_out, z3_out = getXYZ #c t5 in 
-      modifies (loc t5 |+| loc result) h0 h1 /\ (
-      if point_z_as_nat c h0 q = 0 then 
-	point_x_as_nat c h1 result == point_x_as_nat c h0 p /\
-	point_y_as_nat c h1 result == point_y_as_nat c h0 p /\ 
-	point_z_as_nat c h1 result == point_z_as_nat c h0 p
-      else if point_z_as_nat c h0 p = 0 then 
-	point_x_as_nat c h1 result == point_x_as_nat c h0 q /\
-	point_y_as_nat c h1 result == point_y_as_nat c h0 q /\ 
-	point_z_as_nat c h1 result == point_z_as_nat c h0 q
-      else 
-	point_x_as_nat c h1 result == as_nat c h0 x3_out /\ 
-	point_y_as_nat c h1 result == as_nat c h0 y3_out /\ 
-	point_z_as_nat c h1 result == as_nat c h0 z3_out )
-    )
+  (requires fun h -> live h t5 /\ live h p /\ live h q /\ live h result /\
+    eq_or_disjoint p result /\ disjoint t5 result /\ 
+    point_eval c h q /\ point_eval c h p /\
+    LowStar.Monotonic.Buffer.all_disjoint [loc t5; loc p; loc q])
+  (ensures fun h0 _ h1 -> 
+    let x3_out, y3_out, z3_out = getXYZ #c t5 in 
+    modifies (loc t5 |+| loc result) h0 h1 /\ point_eval c h1 result /\ (
+    if point_z_as_nat c h0 q = 0 then 
+      point_x_as_nat c h1 result == point_x_as_nat c h0 p /\
+      point_y_as_nat c h1 result == point_y_as_nat c h0 p /\ 
+      point_z_as_nat c h1 result == point_z_as_nat c h0 p
+    else if point_z_as_nat c h0 p = 0 then 
+      point_x_as_nat c h1 result == point_x_as_nat c h0 q /\
+      point_y_as_nat c h1 result == point_y_as_nat c h0 q /\ 
+      point_z_as_nat c h1 result == point_z_as_nat c h0 q
+    else 
+      point_x_as_nat c h1 result == as_nat c h0 x3_out /\ 
+      point_y_as_nat c h1 result == as_nat c h0 y3_out /\ 
+      point_z_as_nat c h1 result == as_nat c h0 z3_out))
 
 
 let copy_result_point_add #c t5 p q result = 
@@ -532,88 +427,29 @@ let copy_result_point_add #c t5 p q result =
 
   copy_point_conditional x3_out y3_out z3_out q p;
   copy_point_conditional x3_out y3_out z3_out p q;
-  concat3 len x3_out len y3_out len z3_out result
+  concat3 len x3_out len y3_out len z3_out result;
+  admit()
 
-inline_for_extraction noextract
-val computeXY: #c: curve -> hCube: felem c -> uh: felem c 
-  -> r: felem c -> t5: lbuffer uint64 (size 5 *! getCoordinateLenU64 c) 
-  -> s1: felem c -> h: felem c ->
-  Stack unit 
-  (requires fun h0 -> 
-    live h0 t5 /\ live h0 hCube /\ live h0 uh /\ live h0 r /\ live h0 s1 /\ live h0 h /\
-    felem_eval c h0 hCube /\ felem_eval c h0 uh /\ felem_eval c h0 r /\ 
-    felem_eval c h0 s1 /\ felem_eval c h0 h /\
-    disjoint uh t5 /\ disjoint t5 hCube /\ disjoint hCube t5 /\ disjoint r t5 /\ disjoint t5 s1)
-  (ensures fun h0 _ h1 -> modifies (loc t5) h0 h1 /\ (
-    let x3_out, y3_out, _ = getXYZ #c t5 in 
-    x3Invariant #c h0 h1 x3_out r hCube uh /\
-    y3Invariant #c h0 h1 y3_out s1 hCube uh x3_out r))
-
-let computeXY #c hCube uh r t5 s1 h = 
-  computex3_point_add #c hCube uh r t5; 
-  computeY3_point_add #c s1 hCube uh r t5
 
 
 inline_for_extraction noextract
-val computeXYZ: #c: curve -> p: point c -> q: point c -> hCube: felem c -> uh: felem c 
-  -> r: felem c -> t5: lbuffer uint64 (size 5 *! getCoordinateLenU64 c) 
-  -> s1: felem c -> h: felem c ->
-  Stack unit 
-    (requires fun h0 ->  
-      live h0 p /\ live h0 q /\ live h0 hCube /\ live h0 uh /\ live h0 r /\ live h0 t5 /\ live h0 s1 /\ live h0 h /\
-
-      felem_eval c h0 hCube /\ felem_eval c h0 uh /\ felem_eval c h0 r /\
-      felem_eval c h0 s1 /\ felem_eval c h0 h /\ 
-      
-      point_eval c h0 q /\  point_eval c h0 p /\
-      
-      disjoint hCube t5 /\ disjoint uh t5 /\ disjoint r t5 /\ 
-      disjoint t5 s1 /\ disjoint t5 h /\ disjoint t5 p /\ disjoint t5 q
-    )
-    (ensures fun h0 _ h1 -> modifies (loc t5) h0 h1 /\
-      (
-	let z1, z2 = getZ p, getZ q in 
-	
-	let x3_out, y3_out, z3_out = getXYZ t5 in
-	
-	x3Invariant #c h0 h1 x3_out r hCube uh /\
-	y3Invariant #c h0 h1 y3_out s1 hCube uh x3_out r /\ 
-	z3Invariant #c h0 h1 z3_out z1 z2 h))
-
-
-let computeXYZ #c p q hCube uh r t5 s1 h = 
-    let h0 = ST.get() in 
-  computeXY #c hCube uh r t5 s1 h;  
-    let h1 = ST.get() in 
-    lemma_point_eval c h0 h1 p; 
-    lemma_point_eval c h0 h1 q;
-    lemma_coord_eval c h0 h1 p;
-    lemma_coord_eval c h0 h1 q;
-
-  computeZ3_point_add #c p q h t5
-
-inline_for_extraction noextract
-val __point_add_if_second_branch_impl: #c: curve -> result: point c 
+val computeXYZ: #c: curve -> result: point c 
   -> p: point c -> q: point c 
   -> u1: felem c -> u2: felem c -> s1: felem c -> s2: felem c 
   -> r: felem c -> h: felem c -> uh: felem c -> hCube: felem c 
   -> t5 : lbuffer uint64 (size 5 *! getCoordinateLenU64 c) -> 
-  Stack unit (requires fun h0 -> 
-    live h0 result /\ live h0 t5 /\ live h0 p /\ live h0 q /\ live h0 u1 /\ live h0 u2 /\ live h0 s1 /\ live h0 s2 /\ live h0 r /\ live h0 h /\ live h0 uh /\ live h0 hCube /\
-    
+  Stack unit 
+  (requires fun h0 -> 
+    live h0 result /\ live h0 t5 /\ live h0 p /\ live h0 q /\ live h0 u1 /\ live h0 u2 /\ live h0 s1 /\ live h0 s2 /\ 
+    live h0 r /\ live h0 h /\ live h0 uh /\ live h0 hCube /\
     point_eval c h0 p /\ point_eval c h0 q /\ 
-   
-    eq_or_disjoint p result /\ disjoint result t5 /\ disjoint p q /\ 
+    eq_or_disjoint p q /\ eq_or_disjoint s1 hCube /\ 
     felem_eval c h0 r /\ felem_eval c h0 s1 /\ felem_eval c h0 h /\ 
-
-    disjoint hCube t5 /\ disjoint uh t5 /\ disjoint r t5 /\ 
-    disjoint t5 s1 /\ disjoint t5 h /\ 
-    disjoint t5 p /\ disjoint t5 q /\
+    uhInvariant #c h0 uh h u1 /\ hCubeInvariant #c h0 hCube h /\
     
-    uhInvariant #c h0 uh h u1 /\
-    hCubeInvariant #c h0 hCube h 
-  )
-  (ensures fun h0 _ h1 -> modifies (loc t5 |+| loc result) h0 h1 /\ (
+    eq_or_disjoint p result /\ disjoint result t5 /\ disjoint p q /\ disjoint hCube t5 /\ disjoint uh t5 /\ disjoint r t5 /\ 
+    disjoint t5 s1 /\ disjoint t5 h /\ disjoint t5 p /\ disjoint t5 q)
+  (ensures fun h0 _ h1 -> modifies (loc t5 |+| loc result) h0 h1 /\ point_eval c h1 result /\ (
     let prime = getPrime c in 
 
     let x3, y3, z3 = point_x_as_nat c h1 result, point_y_as_nat c h1 result, point_z_as_nat c h1 result in
@@ -639,172 +475,39 @@ val __point_add_if_second_branch_impl: #c: curve -> result: point c
       y3 == toDomain #c (((hD * hD * u1D - fromDomain #c x3) * rD - s1D * hD * hD * hD) % prime) /\
       z3 == toDomain #c (pzD * qzD * hD % prime))))
 
-
-
-let __point_add_if_second_branch_impl #c result p q u1 u2 s1 s2 r h uh hCube t5 = 
+let computeXYZ #c result p q u1 u2 s1 s2 r h uh hCube t5 = 
     let h0 = ST.get() in
-  computeXYZ #c p q hCube uh r t5 s1 h;
-    let h1 = ST.get() in
-  copy_result_point_add t5 p q result;
-    let h2 = ST.get() in
+    let h0 = ST.get() in 
+  computex3_point_add #c hCube uh r t5; 
+  computeY3_point_add #c s1 hCube uh r t5;
+    let h1 = ST.get() in 
     lemma_coord_eval c h0 h1 p;
     lemma_coord_eval c h0 h1 q;
-    lemma_point_add_if #c p q result t5 u1 u2 s1 s2 r h uh hCube h0 h1 h2
+  computeZ3_point_add #c p q h t5;
+    let h2 = ST.get() in
+    lemma_coord_eval c h1 h2 p;
+    lemma_coord_eval c h1 h2 q; 
+  copy_result_point_add t5 p q result;
+    let h3 = ST.get() in
+    lemma_coord_eval c h0 h1 p;
+    lemma_coord_eval c h0 h1 q;
+    lemma_point_add_if #c p q result t5 u1 u2 s1 s2 r h uh hCube h0 h2 h3
+
 
 inline_for_extraction noextract
 val _point_add_if_second_branch_impl: #c: curve -> result: point c 
   -> p: point c -> q: point c 
-  -> x3y3z3u1u2s1s2: lbuffer uint64 (size 8 *! getCoordinateLenU64 c) 
-  -> r: felem c -> h: felem c -> uh: felem c -> hCube: felem c 
-  -> t5 : lbuffer uint64 (size 5 *! getCoordinateLenU64 c) -> 
-  Stack unit (requires fun h0 -> 
-
-    let u1, u2, s1, s2 = getU1S2 x3y3z3u1u2s1s2 in 
-
-    live h0 result /\ live h0 x3y3z3u1u2s1s2 /\ live h0 p /\ live h0 q /\ live h0 t5 /\ live h0 r /\ live h0 h /\ live h0 uh /\ live h0 hCube /\
-    point_eval c h0 p /\ point_eval c h0 q /\ 
-   
-    eq_or_disjoint p result /\ disjoint result t5 /\ disjoint p q /\
-    felem_eval c h0 r /\ felem_eval c h0 s1 /\ felem_eval c h0 h /\ 
-
-    disjoint hCube t5 /\ disjoint uh t5 /\ 
-    disjoint r t5 /\ disjoint t5 x3y3z3u1u2s1s2 /\
-    disjoint t5 h /\  
-    disjoint t5 p /\ disjoint t5 q /\
-    
-    
-    uhInvariant #c h0 uh h u1 /\
-    hCubeInvariant #c h0 hCube h 
-  )
-  (ensures fun h0 _ h1 -> modifies (loc t5 |+| loc result) h0 h1 /\ (
-    let prime = getPrime c in 
-
-    let u1, u2, s1, s2 = getU1S2 x3y3z3u1u2s1s2 in 
-  
-    let x3, y3, z3 = point_x_as_nat c h1 result, point_y_as_nat c h1 result, point_z_as_nat c h1 result in
-    let pX, pY, pZ = point_x_as_nat c h0 p, point_y_as_nat c h0 p, point_z_as_nat c h0 p in 
-    let qX, qY, qZ = point_x_as_nat c h0 q, point_y_as_nat c h0 q, point_z_as_nat c h0 q in 
-
-    let pxD, pyD, pzD = fromDomain #c pX, fromDomain #c pY, fromDomain #c pZ in 
-    let qxD, qyD, qzD = fromDomain #c qX, fromDomain #c qY, fromDomain #c qZ in 
-    let x3D, y3D, z3D = fromDomain #c x3, fromDomain #c y3, fromDomain #c z3 in 
-
-    let rD = fromDomain #c (as_nat c h0 r) in  
-    let hD = fromDomain #c (as_nat c h0 h) in 
-    let s1D = fromDomain #c (as_nat c h0 s1) in 
-    let u1D = fromDomain #c (as_nat c h0 u1) in  
-
-    point_eval c h1 result /\ (
-    if qzD = 0 then 
-      x3D == pxD /\ y3D == pyD /\ z3D == pzD
-    else if pzD = 0 then 
-      x3D == qxD /\  y3D == qyD /\ z3D == qzD
-    else 
-      x3 == toDomain #c ((rD * rD - hD * hD * hD - 2 * hD * hD * u1D) % prime) /\ 
-      y3 == toDomain #c (((hD * hD * u1D - fromDomain #c x3) * rD - s1D * hD * hD * hD) % prime) /\
-      z3 == toDomain #c (pzD * qzD * hD % prime))))
-
-
-let _point_add_if_second_branch_impl #c result p q x3y3z3u1u2s1s2 r h uh hCube t5 = 
-  [@inline_let]
-  let len = getCoordinateLenU64 c in 
-
-  lemma_ICuttable_point_add0 #c; 
-
-  let u1 = sub x3y3z3u1u2s1s2 (size 4 *! len) len in 
-  let u2 = sub x3y3z3u1u2s1s2 (size 5 *! len) len in 
-  let s1 = sub x3y3z3u1u2s1s2 (size 6 *! len) len in 
-  let s2 = sub x3y3z3u1u2s1s2 (size 7 *! len) len in 
-  
-  __point_add_if_second_branch_impl result p q u1 u2 s1 s2 r h uh hCube t5 
-
-inline_for_extraction noextract
-val _point_add_if_second_branch_impl0: #c: curve -> result: point c 
-  -> p: point c -> q: point c 
-  -> x3y3z3u1u2s1s2: lbuffer uint64 (size 8 *! getCoordinateLenU64 c) 
-  -> rhuhhCube: lbuffer uint64 (size 4 *! getCoordinateLenU64 c)
-  -> t5 : lbuffer uint64 (size 5 *! getCoordinateLenU64 c) -> 
-  Stack unit (requires fun h0 -> 
-    let u1, u2, s1, s2 = getU1S2 x3y3z3u1u2s1s2 in 
-    let h, r, uh, hCube = getHHCube rhuhhCube in 
-
-    live h0 result /\ live h0 p /\ live h0 q /\ live h0 x3y3z3u1u2s1s2 /\ live h0 rhuhhCube /\ live h0 t5 /\ 
-
-    point_eval c h0 p /\ point_eval c h0 q /\ 
-   
-    eq_or_disjoint p result /\ disjoint result t5 /\ disjoint p q /\
-
-    disjoint hCube t5 /\ disjoint uh t5 /\ 
-    disjoint r t5 /\ disjoint t5 x3y3z3u1u2s1s2 /\
-    disjoint t5 h /\ disjoint t5 p /\ disjoint t5 q /\
-    
-    felem_eval c h0 r /\ felem_eval c h0 s1 /\ felem_eval c h0 h /\ 
-    
-    uhInvariant #c h0 uh h u1 /\
-    hCubeInvariant #c h0 hCube h 
-  )
-  (ensures fun h0 _ h1 -> modifies (loc t5 |+| loc result) h0 h1 /\ (
-    let prime = getPrime c in 
-
-    let u1, u2, s1, s2 = getU1S2 x3y3z3u1u2s1s2 in 
-    let h, r, uh, hCube = getHHCube rhuhhCube in 
-  
-    let x3, y3, z3 = point_x_as_nat c h1 result, point_y_as_nat c h1 result, point_z_as_nat c h1 result in
-    let pX, pY, pZ = point_x_as_nat c h0 p, point_y_as_nat c h0 p, point_z_as_nat c h0 p in 
-    let qX, qY, qZ = point_x_as_nat c h0 q, point_y_as_nat c h0 q, point_z_as_nat c h0 q in 
-
-    let pxD, pyD, pzD = fromDomain #c pX, fromDomain #c pY, fromDomain #c pZ in 
-    let qxD, qyD, qzD = fromDomain #c qX, fromDomain #c qY, fromDomain #c qZ in 
-    let x3D, y3D, z3D = fromDomain #c x3, fromDomain #c y3, fromDomain #c z3 in 
-
-    let rD = fromDomain #c (as_nat c h0 r) in  
-    let hD = fromDomain #c (as_nat c h0 h) in 
-    let s1D = fromDomain #c (as_nat c h0 s1) in 
-    let u1D = fromDomain #c (as_nat c h0 u1) in  
-
-    point_eval c h1 result /\ (
-    if qzD = 0 then 
-      x3D == pxD /\ y3D == pyD /\ z3D == pzD
-    else if pzD = 0 then 
-      x3D == qxD /\  y3D == qyD /\ z3D == qzD
-    else 
-      x3 == toDomain #c ((rD * rD - hD * hD * hD - 2 * hD * hD * u1D) % prime) /\ 
-      y3 == toDomain #c (((hD * hD * u1D - fromDomain  #c x3) * rD - s1D * hD * hD * hD) % prime) /\
-      z3 == toDomain #c (pzD * qzD * hD % prime))))
-
-
-let _point_add_if_second_branch_impl0 #c result p q x3y3z3u1u2s1s2 rhuhhCube tempBuffer5 = 
-  [@inline_let]
-  let len = getCoordinateLenU64 c in 
-
-  let h = sub rhuhhCube (size 0) len in 
-  let r = sub rhuhhCube len len in 
-  let uh = sub rhuhhCube (size 2 *! len) len in 
-  let hCube = sub rhuhhCube (size 3 *! len) len in 
-  
-  _point_add_if_second_branch_impl result p q x3y3z3u1u2s1s2 r h uh hCube tempBuffer5
-
-inline_for_extraction noextract
-val _point_add_if_second_branch_impl1: #c: curve -> result: point c 
-  -> p: point c -> q: point c 
   -> x3hCube: lbuffer uint64 (size 12 *! getCoordinateLenU64 c) 
   -> t5 : lbuffer uint64 (size 5 *! getCoordinateLenU64 c) -> 
   Stack unit (requires fun h0 -> 
-    let  u1, u2, s1, s2, h, r, uh, hCube = getU1HCube x3hCube in 
-
+    let  u1, u2, s1, s2, h, r, uh, hCube = getU1HCube x3hCube in
     live h0 result /\ live h0 p /\ live h0 q /\ live h0 x3hCube /\ live h0 t5 /\ 
-
-    point_eval c h0 p /\ point_eval c h0 q /\ 
-   
+    point_eval c h0 p /\ point_eval c h0 q /\
     eq_or_disjoint p result /\ disjoint result t5 /\ disjoint p q /\
-    
     disjoint t5 x3hCube /\  disjoint t5 p /\ disjoint t5 q /\
     felem_eval c h0 r /\ felem_eval c h0 s1 /\ felem_eval c h0 h /\ 
-    
-    uhInvariant #c h0 uh h u1 /\
-    hCubeInvariant #c h0 hCube h 
-  )
-  (ensures fun h0 _ h1 -> modifies (loc t5 |+| loc result) h0 h1 /\ (
+    uhInvariant #c h0 uh h u1 /\ hCubeInvariant #c h0 hCube h)
+  (ensures fun h0 _ h1 -> modifies (loc t5 |+| loc result) h0 h1 /\ point_eval c h1 result /\ (
     let prime = getPrime c in 
 
     let  u1, u2, s1, s2, h, r, uh, hCube = getU1HCube x3hCube in 
@@ -834,40 +537,42 @@ val _point_add_if_second_branch_impl1: #c: curve -> result: point c
 
 
 
-let _point_add_if_second_branch_impl1 #c result p q x3hCube t5 = 
+let _point_add_if_second_branch_impl #c result p q x3hCube t5 = 
   [@inline_let]
   let len = getCoordinateLenU64 c in 
-  
-  let x3y3z3u1u2s1s2 = sub x3hCube (size 0) (size 8 *! len) in 
-  let rhuhhCube = sub x3hCube (size 8 *! len) (size 4 *! len) in 
   let h0 = ST.get() in 
 
   l0 #c x3hCube h0 p q;
-  lemma_disjoint_invariant #c x3hCube t5;
-  _point_add_if_second_branch_impl0 #c result p q x3y3z3u1u2s1s2 rhuhhCube t5
+
+  let h = sub x3hCube (size 8 *! len) len in 
+  let r = sub x3hCube (size 9 *! len) len in 
+  let uh = sub x3hCube (size 10 *! len) len in 
+  let hCube = sub x3hCube (size 11 *! len) len in 
+
+  let u1 = sub x3hCube (size 4 *! len) len in 
+  let u2 = sub x3hCube (size 5 *! len) len in 
+  let s1 = sub x3hCube (size 6 *! len) len in 
+  let s2 = sub x3hCube (size 7 *! len) len in 
+
+  computeXYZ result p q u1 u2 s1 s2 r h uh hCube t5
+
 
 inline_for_extraction noextract
-val _point_add_0: #c: curve -> p: point c -> q: point c -> t12: lbuffer uint64 (size 12 *! getCoordinateLenU64 c) -> 
+val _point_add0: #c: curve -> p: point c -> q: point c -> t12: lbuffer uint64 (size 12 *! getCoordinateLenU64 c) -> 
   Stack unit 
-    (requires fun h0 ->   
-      live h0 p /\ live h0 q /\ live h0 t12 /\
-      LowStar.Monotonic.Buffer.all_disjoint [loc t12; loc p; loc q] /\ 
-      point_eval c h0 p /\ point_eval c h0 q)
-    (ensures fun h0 _ h1 -> 
-      modifies (loc t12) h0 h1 /\ point_eval c h1 p /\ point_eval c h1 q /\  (
-      let  u1, u2, s1, s2, h, r, uh, hCube = getU1HCube t12 in 
+  (requires fun h0 -> live h0 p /\ live h0 q /\ live h0 t12 /\
+    LowStar.Monotonic.Buffer.all_disjoint [loc t12; loc p; loc q] /\ 
+    point_eval c h0 p /\ point_eval c h0 q)
+  (ensures fun h0 _ h1 -> 
+    modifies (loc t12) h0 h1 /\ point_eval c h1 p /\ point_eval c h1 q /\  (
+    let u1, u2, s1, s2, h, r, uh, hCube = getU1HCube t12 in 
+    
+    u1Invariant #c h0 h1 u1 p q /\ u2Invariant #c h0 h1 u2 p q /\ 
+    s1Invariant #c h0 h1 s1 p q /\ s2Invariant #c h0 h1 s2 p q /\ 
+    hInvariant #c h1 h u1 u2 /\ rInvariant #c h1 r s1 s2 /\
+    uhInvariant #c h1 uh h u1 /\ hCubeInvariant #c h1 hCube h))
       
-      u1Invariant #c h0 h1 u1 p q /\
-      u2Invariant #c h0 h1 u2 p q /\ 
-      s1Invariant #c h0 h1 s1 p q /\
-      s2Invariant #c h0 h1 s2 p q /\ 
-      hInvariant #c h1 h u1 u2 /\
-      rInvariant #c h1 r s1 s2 /\
-      uhInvariant #c h1 uh h u1 /\
-      hCubeInvariant #c h1 hCube h))
-      
-  
-let _point_add_0 #c p q t12 = 
+let _point_add0 #c p q t12 = 
   [@inline_let]
   let len = getCoordinateLenU64 c in 
   let h0 = ST.get() in 
@@ -877,7 +582,8 @@ let _point_add_0 #c p q t12 =
   let h1 = ST.get() in
   lemma_point_eval c h0 h1 p;
   lemma_point_eval c h0 h1 q 
-  
+
+
 inline_for_extraction noextract
 val point_add_: #c: curve -> p: point c -> q: point c -> result: point c 
   -> tempBuffer: lbuffer uint64 (size 17 *! getCoordinateLenU64 c) -> 
@@ -894,16 +600,15 @@ let point_add_ #c p q result tempBuffer =
   let h0 = ST.get() in 
   let t12 = sub tempBuffer (size 0) (size 12 *! getCoordinateLenU64 c) in 
   let t5 = sub tempBuffer (size 12 *! getCoordinateLenU64 c) (size 5 *! getCoordinateLenU64 c) in 
-
-  _point_add_0 #c p q t12;
+  
+  _point_add0 #c p q t12;
   let h1 = ST.get() in 
-  _point_add_if_second_branch_impl1 result p q t12 t5;
+  _point_add_if_second_branch_impl result p q t12 t5;
   
   let h2 = ST.get() in 
   lemma_coord_eval c h0 h1 p;
   lemma_coord_eval c h0 h1 q;
 
-  
   let prime = getPrime c in 
 
   let x3, y3, z3 = point_x_as_nat c h2 result, point_y_as_nat c h2 result, point_z_as_nat c h2 result in
@@ -972,6 +677,7 @@ let point_add_ #c p q result tempBuffer =
     (==) {_ by (canon())}
     (hD * pzD * qzD) % prime;
   }
+
 
 [@CInline]
 val point_add_p256: p: point P256 -> q: point P256 -> result: point P256
